imp/Imp2CsharpminorSim.v
@@ -1,4 +1,4 @@
-From compcert Require Import Smallstep Clight Integers Events Behaviors Errors.
+From compcert Require Import Smallstep AST Integers Events Behaviors Errors.
 Require Import Coqlib.
 Require Import ITreelib.
 Require Import Universe.
@@ -10,118 +10,102 @@ Require Import ModSem.
 Require Import Imp.
 Require Import Imp2Csharpminor.
 Require Import ImpProofs.
+Require Import SimSTS2.
 Require Import Mem0.
 Require Import IRed.
 
 Set Implicit Arguments.
 
-Definition single_events_at (L: Smallstep.semantics) (s:L.(Smallstep.state)) : Prop :=
-  forall t s', Step L s t s' -> (t = E0).
+(* Section SIM. *)
 
-Record strict_determinate_at (L: Smallstep.semantics) (s:L.(Smallstep.state)) : Prop :=
-  Strict_determinate_at {
-      ssd_determ_at: forall t1 s1 t2 s2
-        (STEP0: Step L s t1 s1)
-        (STEP1 :Step L s t2 s2),
-        <<EQ: s1 = s2>>;
-    ssd_determ_at_final: forall tr s' retv
-        (FINAL: Smallstep.final_state L s retv)
-        (STEP: Step L s tr s'),
-        False;
-    ssd_traces_at:
-      single_events_at L s
-  }.
+(*   Variable L0: STS.semantics. *)
+(*   Variable L1: Smallstep.semantics. *)
+(*   Variable idx: Type. *)
+(*   Variable ord: idx -> idx -> Prop. *)
 
-Section SIM.
+(*   Local Open Scope smallstep_scope. *)
 
-  Variable L0: STS.semantics.
-  Variable L1: Smallstep.semantics.
-  Variable idx: Type.
-  Variable ord: idx -> idx -> Prop.
+(*   Variant _sim sim (i0 j0: idx) (st_src0: L0.(STS.state)) (st_tgt0: L1.(Smallstep.state)): Prop := *)
+(*   | sim_fin *)
+(*       retv *)
+(*       (RANGE: (0 <= retv <= Int.max_unsigned)%Z) *)
+(*       (SRT: _.(state_sort) st_src0 = final retv) *)
+(*       (SRT: _.(Smallstep.final_state) st_tgt0 (Int.repr retv)) *)
+(*       (DTM: (* sd_final_determ *) *)
+(*          forall (s : Smallstep.state L1) (r1 r2 : int), *)
+(*            Smallstep.final_state L1 s r1 -> Smallstep.final_state L1 s r2 -> r1 = r2) *)
+(*     : *)
+(*       _sim sim i0 j0 st_src0 st_tgt0 *)
 
-  Local Open Scope smallstep_scope.
+(*   | sim_vis *)
+(*       (SRT: _.(state_sort) st_src0 = vis) *)
+(*       (SRT: exists _ev_tgt _st_tgt1, Step L1 st_tgt0 [_ev_tgt] _st_tgt1) *)
+(*       (SIM: forall ev_tgt st_tgt1 *)
+(*           (STEP: Step L1 st_tgt0 ev_tgt st_tgt1) *)
+(*         , *)
+(*           exists st_src1 ev_src (STEP: _.(step) st_src0 (Some ev_src) st_src1), *)
+(*             (<<MATCH: Forall2 match_event ev_tgt [ev_src]>>) /\ *)
+(*             (<<SIM: exists i1 j1, sim i1 j1 st_src1 st_tgt1>>)) *)
+(*     : *)
+(*       _sim sim i0 j0 st_src0 st_tgt0 *)
 
-  Variant _sim sim (i0 j0: idx) (st_src0: L0.(STS.state)) (st_tgt0: L1.(Smallstep.state)): Prop :=
-  | sim_fin
-      retv
-      (RANGE: (0 <= retv <= Int.max_unsigned)%Z)
-      (SRT: _.(state_sort) st_src0 = final retv)
-      (SRT: _.(Smallstep.final_state) st_tgt0 (Int.repr retv))
-      (DTM: (* sd_final_determ *)
-         forall (s : Smallstep.state L1) (r1 r2 : int),
-           Smallstep.final_state L1 s r1 -> Smallstep.final_state L1 s r2 -> r1 = r2)
-    :
-      _sim sim i0 j0 st_src0 st_tgt0
+(*   | sim_demonic_src *)
+(*       (SRT: _.(state_sort) st_src0 = demonic) *)
+(*       (SIM: exists st_src1 *)
+(*           (STEP: _.(step) st_src0 None st_src1) *)
+(*         , *)
+(*           exists i1, <<ORD: ord i1 i0>> /\ <<SIM: exists j1, sim i1 j1 st_src1 st_tgt0>>) *)
+(*     : *)
+(*       _sim sim i0 j0 st_src0 st_tgt0 *)
 
-  | sim_vis
-      (SRT: _.(state_sort) st_src0 = vis)
-      (SRT: exists _ev_tgt _st_tgt1, Step L1 st_tgt0 [_ev_tgt] _st_tgt1)
-      (SIM: forall ev_tgt st_tgt1
-          (STEP: Step L1 st_tgt0 ev_tgt st_tgt1)
-        ,
-          exists st_src1 ev_src (STEP: _.(step) st_src0 (Some ev_src) st_src1),
-            (<<MATCH: Forall2 match_event ev_tgt [ev_src]>>) /\
-            (<<SIM: exists i1 j1, sim i1 j1 st_src1 st_tgt1>>))
-    :
-      _sim sim i0 j0 st_src0 st_tgt0
+(*   | sim_demonic_tgt_dtm *)
+(*       (*** WRONG DEF, Note: UB in tgt ***) *)
+(*       (* (SIM: forall st_tgt1 *) *)
+(*       (*     (STEP: Step L1 st_tgt0 E0 st_tgt1) *) *)
+(*       (*   , *) *)
+(*       (*     exists i1, <<ORD: ord i1 i0>> /\ <<SIM: sim i1 st_src0 st_tgt1>>) *) *)
+(*       (DTM: strict_determinate_at L1 st_tgt0) *)
+(*       (SIM: exists st_tgt1 *)
+(*           (STEP: Step L1 st_tgt0 E0 st_tgt1) *)
+(*         , *)
+(*           exists j1, <<ORD: ord j1 j0>> /\ <<SIM: exists i1, sim i1 j1 st_src0 st_tgt1>>) *)
+(*       (*** equivalent def ***) *)
+(*       (* st_tgt1 *) *)
+(*       (* (STEP: Step L1 st_tgt0 E0 st_tgt1) *) *)
+(*       (* i1 *) *)
+(*       (* (ORD: ord i1 i0) *) *)
+(*       (* (SIM: sim i1 st_src0 st_tgt1) *) *)
+(*     : *)
+(*       _sim sim i0 j0 st_src0 st_tgt0 *)
 
-  | sim_demonic_src
-      (SRT: _.(state_sort) st_src0 = demonic)
-      (SIM: exists st_src1
-          (STEP: _.(step) st_src0 None st_src1)
-        ,
-          exists i1, <<ORD: ord i1 i0>> /\ <<SIM: exists j1, sim i1 j1 st_src1 st_tgt0>>)
-    :
-      _sim sim i0 j0 st_src0 st_tgt0
+(*   | sim_angelic_src *)
+(*       (SRT: _.(state_sort) st_src0 = angelic) *)
+(*       (SIM: forall st_src1 *)
+(*           (STEP: _.(step) st_src0 None st_src1) *)
+(*         , *)
+(*           exists i1, <<ORD: ord i1 i0>> /\ <<SIM: exists j1, sim i1 j1 st_src1 st_tgt0>>) *)
+(*     : *)
+(*       _sim sim i0 j0 st_src0 st_tgt0 *)
+(*   . *)
 
-  | sim_demonic_tgt_dtm
-      (*** WRONG DEF, Note: UB in tgt ***)
-      (* (SIM: forall st_tgt1 *)
-      (*     (STEP: Step L1 st_tgt0 E0 st_tgt1) *)
-      (*   , *)
-      (*     exists i1, <<ORD: ord i1 i0>> /\ <<SIM: sim i1 st_src0 st_tgt1>>) *)
-      (DTM: strict_determinate_at L1 st_tgt0)
-      (SIM: exists st_tgt1
-          (STEP: Step L1 st_tgt0 E0 st_tgt1)
-        ,
-          exists j1, <<ORD: ord j1 j0>> /\ <<SIM: exists i1, sim i1 j1 st_src0 st_tgt1>>)
-      (*** equivalent def ***)
-      (* st_tgt1 *)
-      (* (STEP: Step L1 st_tgt0 E0 st_tgt1) *)
-      (* i1 *)
-      (* (ORD: ord i1 i0) *)
-      (* (SIM: sim i1 st_src0 st_tgt1) *)
-    :
-      _sim sim i0 j0 st_src0 st_tgt0
+(*   Definition sim: _ -> _ -> _ -> _ -> Prop := paco4 _sim bot4. *)
 
-  | sim_angelic_src
-      (SRT: _.(state_sort) st_src0 = angelic)
-      (SIM: forall st_src1
-          (STEP: _.(step) st_src0 None st_src1)
-        ,
-          exists i1, <<ORD: ord i1 i0>> /\ <<SIM: exists j1, sim i1 j1 st_src1 st_tgt0>>)
-    :
-      _sim sim i0 j0 st_src0 st_tgt0
-  .
+(*   Lemma sim_mon: monotone4 _sim. *)
+(*   Proof. *)
+(*     ii. inv IN. *)
 
-  Definition sim: _ -> _ -> _ -> _ -> Prop := paco4 _sim bot4.
+(*     - econs 1; et. *)
+(*     - econs 2; et. i. exploit SIM; et. i; des. esplits; et. *)
+(*     - econs 3; et. des. esplits; et. *)
+(*     - econs 4; et. des. esplits; et. *)
+(*     - econs 5; et. i. exploit SIM; et. i; des. esplits; et. *)
+(*   Qed. *)
 
-  Lemma sim_mon: monotone4 _sim.
-  Proof.
-    ii. inv IN.
+(* End SIM. *)
 
-    - econs 1; et.
-    - econs 2; et. i. exploit SIM; et. i; des. esplits; et.
-    - econs 3; et. des. esplits; et.
-    - econs 4; et. des. esplits; et.
-    - econs 5; et. i. exploit SIM; et. i; des. esplits; et.
-  Qed.
-
-End SIM.
-
-Hint Constructors _sim.
-Hint Unfold sim.
-Hint Resolve sim_mon: paco.
+(* Hint Constructors _sim. *)
+(* Hint Unfold sim. *)
+(* Hint Resolve sim_mon: paco. *)
 
 Lemma unbind_trigger E:
   forall [X0 X1 A : Type] (ktr0 : X0 -> itree E A) (ktr1 : X1 -> itree E A) e0 e1,
@@ -145,20 +129,15 @@ Proof.
   des. clarify.
 Qed.
 
+From compcert Require Import Csharpminor.
+
 Section PROOF.
 
-  From compcert Require Import Csharpminor.
   Import ModSemL.
 
   Context `{Σ: GRA.t}.
 
   Definition ordN : nat -> nat -> Prop := fun a b => True.
-
-  Ltac sim_red := Red.prw ltac:(_red_gen) 2 0.
-  Ltac sim_tau := (try sim_red); econs 3; ss; clarify; eexists; exists (step_tau _); eexists; split; auto; eexists.
-
-  Ltac sim_triggerUB := pfold; ss; unfold triggerUB; (try sim_red); econs 5; i; ss; auto;
-                        dependent destruction STEP; try (irw in x; clarify; fail).
 
   Lemma map_val_vadd_comm
         a b v
@@ -197,11 +176,17 @@ Section PROOF.
         rewrite Z.mod_mod; try nia. rewrite Z.mod_small; try nia.
   Qed.
 
+  Ltac sim_red := Red.prw ltac:(_red_gen) 2 0.
+  Ltac sim_tau := (try sim_red); econs 3; ss; clarify; eexists; exists (step_tau _); eexists; split; auto.
+
+  Ltac sim_triggerUB := pfold; ss; unfold triggerUB; (try sim_red); econs 5; i; ss; auto;
+                        dependent destruction STEP; try (irw in x; clarify; fail).
+
   Lemma step_expr
         e te
         tcode tf tcont tge tle tm (src: ModL.t) (tgt: Csharpminor.program)
         r ms mn ge le rstate pstate ktr
-        i0 j0 i1 j1
+        i0 i1
         (MLE: match_le le tle)
         (CEXP: compile_expr e = Some te)
         (SIM:
@@ -209,11 +194,11 @@ Section PROOF.
              wf_val rv ->
              eval_expr tge empty_env tle tm te trv ->
              trv = map_val rv ->
-             paco4 (_sim (ModL.compile src) (semantics tgt) ordN) r i1 j1
+             paco3 (_sim (ModL.compile src) (semantics tgt) ordN) r i1
                    (ktr (rstate, pstate, (le, rv)))
                    (State tf tcode tcont empty_env tle tm))
     :
-      paco4 (_sim (ModL.compile src) (semantics tgt) ordN) r i0 j0
+      paco3 (_sim (ModL.compile src) (semantics tgt) ordN) r i0
             (r0 <- EventsL.interp_Es (prog ms) (transl_all mn (interp_imp ge (denote_expr e) le)) (rstate, pstate);; ktr r0)
             (State tf tcode tcont empty_env tle tm).
   Proof.
@@ -223,18 +208,19 @@ Section PROOF.
     generalize dependent e. Local Opaque Init.Nat.add. induction e; i; ss; des; clarify.
     - rewrite interp_imp_expr_Var. sim_red.
       destruct (alist_find v le) eqn:AFIND; try sim_red.
-      + pfold. repeat (sim_tau; left; pfold). sim_red.
-        unfold assume. grind. econs 5; ss; auto. i. eapply angelic_step in STEP; des; clarify.
-        eexists; split; auto. eexists. left. pfold.
-        do 5 (sim_tau; left; pfold). sim_tau. left.
+      + repeat (pfold; sim_tau; left). sim_red.
+        unfold assume. grind.
+        pfold. econs 5; ss; auto. i. eapply angelic_step in STEP; des; clarify.
+        eexists; split; auto. left.
+        do 6 (pfold; sim_tau; left).
         sim_red. eapply SIM; auto.
         econs. inv MLE. specialize ML with (x:=v) (sv:=(Some v0)).
         hexploit ML; auto. i. des. ss. clarify.
       + sim_triggerUB.
     - rewrite interp_imp_expr_Lit.
       sim_red. unfold assume. grind. pfold. econs 5; auto. i. eapply angelic_step in STEP; des; clarify.
-      eexists; split; auto. eexists. left; pfold.
-      do 5 (sim_tau; left; pfold). sim_tau. left.
+      eexists; split; auto. left.
+      do 6 (pfold; sim_tau; left).
       sim_red. eapply SIM; eauto. econs. unfold map_val. ss.
     - rewrite interp_imp_expr_Plus.
       sim_red. destruct (compile_expr e1) eqn:EXP1; destruct (compile_expr e2) eqn:EXP2; ss; clarify.
@@ -243,8 +229,8 @@ Section PROOF.
       i. sim_red.
       unfold unwrapU. destruct (vadd rv rv0) eqn:VADD; ss; clarify.
       + sim_red. unfold assume. grind. pfold. econs 5; auto. i. eapply angelic_step in STEP; des; clarify.
-        eexists; split; auto. eexists. left; pfold.
-        do 5 (sim_tau; left; pfold). sim_tau. left.
+        eexists; split; auto. left.
+        do 6 (pfold; sim_tau; left).
         sim_red. specialize SIM with (rv:=v) (trv:= map_val v). apply SIM; auto.
         econs; eauto. ss. f_equal. apply map_val_vadd_comm; auto.
       + sim_triggerUB.
@@ -257,9 +243,8 @@ Section PROOF.
         es tes
         tcode tf tcont tge tle tm (src: ModL.t) (tgt: Csharpminor.program)
         r ms mn ge le rstate pstate ktr
-        i0 j0 i1 j1
-        (IDX1: i0 = (List.length es)*EMI + i1)
-        (IDX2: j0 = (List.length es)*EMI + j1)
+        i0 i1
+        (IDX: i0 = (List.length es)*EMI + i1)
         (MLE: match_le le tle)
         (CEXP: compile_exprs es = Some tes)
         (SIM:
@@ -267,11 +252,11 @@ Section PROOF.
              Forall wf_val rvs ->
              eval_exprlist tge empty_env tle tm tes trvs ->
              trvs = List.map map_val rvs ->
-             paco4 (_sim (ModL.compile src) (semantics tgt) ordN) r i1 j1
+             paco3 (_sim (ModL.compile src) (semantics tgt) ordN) r i1
                    (ktr (rstate, pstate, (le, rvs)))
                    (State tf tcode tcont empty_env tle tm))
     :
-      paco4 (_sim (ModL.compile src) (semantics tgt) ordN) r i0 j0
+      paco3 (_sim (ModL.compile src) (semantics tgt) ordN) r i0
             (r0 <- EventsL.interp_Es (prog ms) (transl_all mn (interp_imp ge (denote_exprs es) le)) (rstate, pstate);; ktr r0)
             (State tf tcode tcont empty_env tle tm).
   Proof.
@@ -285,7 +270,6 @@ Section PROOF.
       rewrite interp_imp_bind. sim_red. eapply step_expr; eauto.
       i. unfold ordN in *. rewrite interp_imp_bind. sim_red.
       eapply IHes.
-      { admit "mid: index". }
       { admit "mid: index". }
       { auto. }
       i. rewrite interp_imp_Ret. sim_red. eapply SIM; eauto.
@@ -301,12 +285,18 @@ Section PROOF.
   (* Let src_sem := ModL.compile (Mod.add_list ([src_mod] ++ [Mem])). *)
   (* Let tgt_sem := semantics2 tgt. *)
 
+  Lemma compile_stmt_no_Sreturn
+        gm src e
+        (CSTMT: compile_stmt gm src = Some (Sreturn e))
+    :
+      False.
+  Proof. destruct src; ss; uo; des_ifs; clarify. Qed.
 
   Theorem match_states_sim
           (src: Imp.program) tgt
           gm ge ms mn
           ist cst
-          i0 j0
+          i0
           (MODNAME: mn = src.(name))
           (GMAP: gm = get_gmap src)
           (MODSEML: ms = (ImpMod.get_modL src).(ModL.enclose))
@@ -314,7 +304,7 @@ Section PROOF.
           (COMP: Imp2Csharpminor.compile src = OK tgt)
           (MS: match_states mmem gm ge ms mn ist cst)
     :
-      <<SIM: sim (ModL.compile (Mod.add_list ([Mem] ++ [ImpMod.get_mod src]))) (semantics tgt) ordN i0 j0 ist cst>>.
+      <<SIM: sim (ModL.compile (Mod.add_list ([Mem] ++ [ImpMod.get_mod src]))) (semantics tgt) ordN i0 ist cst>>.
   Proof.
     move GMAP before ms. move MODSEML before GMAP. move GENV before MODSEML. move COMP before GENV.
     move MODNAME before COMP.
@@ -329,95 +319,56 @@ Section PROOF.
     (* generalize dependent code. *)
     (* induction code; i. *)
     - ss. unfold itree_of_cont_stmt, itree_of_imp_cont.
-      rewrite interp_imp_Skip.
-      destruct tcont eqn:TCONT; ss; clarify.
-      + inv MCONT. inv MSTACK; ss; clarify. unfold idK. sim_red. destruct rp. sim_red.
-        rewrite interp_imp_expr_Var. sim_red.
-        unfold unwrapU.
-        des_ifs; grind.
-        2:{ sim_triggerUB. }
-        repeat (pfold; sim_tau; left). sim_red. unfold assume.
-        pfold. econs 5; ss; auto. grind. eapply angelic_step in STEP; des; clarify.
-        eexists; split; auto. eexists. left.
-        repeat (pfold; sim_tau; left). sim_red.
-        destruct r0. ss. destruct l.
-        { admit "mid: need wf-r_state". }
-        grind. do 2 (pfold; sim_tau; left).
-        (* tau point *)
-        sim_red.
-        pfold. econs 4.
-        { admit "ez: strict_determinate_at". }
-        eexists. eexists.
-        { eapply step_skip_call; ss. }
-        eexists; split; auto. eexists.
-        admit "ez? sim final state".
-      + inv MCONT; clarify.
-        sim_red.
-        (* tau point *)
-        pfold.
-        econs 4; auto.
+      rewrite interp_imp_Skip. ss; clarify.
+      (* move MM before tm. move ML before MM. move tcont before ML. *)
+      (* revert_until ML. *)
+      destruct tcont; ss; clarify.
+      inv MCONT; clarify.
+      { destruct s; ss; clarify.
+        destruct tcont; clarify.
+        - inv MSTACK.
+          + 
+
+
+        sim_red. pfold. econs 6; clarify.
         { admit "ez: strict_determinate_at". }
         eexists. eexists.
         { eapply step_skip_seq. }
-        eexists; split; auto. eexists.
-        right. eapply CIH.
-        eapply match_states_intro with (le0:=le) (rp0:=rp) (code0:=code); eauto.
-      + admit "ez?: should not happen (Kblock should never appear)".
-      + inv MCONT. inv MSTACK; clarify.
-        unfold idK. sim_red. destruct rp. sim_red.
 
-        rewrite interp_imp_expr_Var. sim_red.
-        unfold unwrapU.
-        des_ifs; grind.
-        2:{ sim_triggerUB. }
-        repeat (pfold; sim_tau; left). sim_red. unfold assume.
-        pfold. econs 5; ss; auto. grind. eapply angelic_step in STEP; des; clarify.
-        eexists; split; auto. eexists. left.
-        repeat (pfold; sim_tau; left). sim_red.
-        destruct r0. ss. destruct l.
-        { admit "mid: need wf-r_state". }
-        grind. repeat (pfold; sim_tau; left). sim_red.
 
-        rewrite Any.upcast_downcast. ss. grind.
-        do 2 (pfold; sim_tau; left). sim_red.
-        (* tau point *)
-        pfold. econs 4; auto.
-        { admit "ez: strict_determinate_at". }
-        eexists. eexists.
-        { eapply step_skip_call; ss; clarify; auto. }
-        eexists; split; auto. eexists. left; pfold.
-        econs 4; auto.
-        { admit "ez: strict_determinate_at". }
-        eexists. eexists.
-        { eapply step_return. }
-        eexists; split; auto. eexists. right.
-        apply CIH.
-        hexploit match_states_intro.
-        { instantiate (3:=get_gmap src). instantiate (2:=Skip). ss. }
-        2,3,4,5:eauto.
-        2:{ unfold itree_of_cont_stmt, itree_of_imp_cont. rewrite interp_imp_Skip.
-            rewrite transl_all_ret. rewrite EventsL.interp_Es_ret. grind. eapply H. }
-        { econs. i. exists (map_val_opt sv); split; auto.
-          admit "ez? alist & Maps.PTree". }
+        }
+      sim_red. pfold. econs 6; clarify.
+      { admit "ez: strict_determinate_at". }
+      eexists. eexists.
+      { eapply step_skip_seq. }
+      eexists. eexists (step_tau _). eexists. sim_red. right.
+      destruct rp. eapply CIH.
+      hexploit match_states_intro; eauto.
+      all: (destruct s; eauto).
+      all: (generalize dependent tcont; induction tcont; i; ss; clarify; eauto).
+      all: (eapply compile_stmt_no_Sreturn in CST; clarify).
+
     - ss. unfold itree_of_cont_stmt, itree_of_imp_cont.
       rewrite interp_imp_Assign. sim_red. grind.
       destruct (compile_expr e) eqn:EXP; uo; ss. destruct rp. grind.
       eapply step_expr; eauto. i.
       (* tau point *)
-      do 2 (pfold; sim_tau; left). sim_red.
-      pfold. econs 4; auto.
+      unfold ordN in *.
+      do 1 (pfold; sim_tau; left). sim_red.
+      pfold. econs 6; auto.
       { admit "ez? strict_determinate_at". }
       eexists. eexists.
       { eapply step_set. eapply H0. }
-      unfold ordN in *. eexists; split; eauto; auto.
+      eexists. eexists.
+      { eapply step_tau. }
       eexists. right. apply CIH.
       hexploit match_states_intro.
       { instantiate (2:=Skip). instantiate (2:=get_gmap src). ss. }
-      2,3,4,5:eauto.
-      2:{ unfold itree_of_cont_stmt, itree_of_imp_cont. rewrite interp_imp_Skip.
-          rewrite transl_all_ret. rewrite EventsL.interp_Es_ret. grind. eapply H1. }
+      2,3,4,5,7:eauto.
+      2:{ unfold itree_of_cont_stmt, itree_of_imp_cont. rewrite interp_imp_Skip. ss. }
       { econs. i. exists (map_val_opt sv); split; auto.
         admit "ez? alist & Maps.PTree". }
+
     - unfold itree_of_cont_stmt, itree_of_imp_cont. rewrite interp_imp_Seq. sim_red.
       ss. destruct (compile_stmt (get_gmap src) code1) eqn:CSC1; destruct (compile_stmt (get_gmap src) code2) eqn:CSC2; uo; clarify.
 
@@ -429,22 +380,27 @@ Section PROOF.
         (transl_all (name src) (let (le1, _) := v in interp_imp (Sk.load_skenv (defs src)) (denote_stmt code2) le1)) st1);; next x)).
 
       (* tau point *)
-      pfold. econs 4.
+      pfold. econs 6; ss; clarify.
       { admit "ez: strict_determinate_at". }
       eexists. eexists.
       { eapply step_seq. }
-      eexists; split; auto. eexists. right. eapply CIH.
+      eexists. eexists.
+      { eapply step_tau. }
+      eexists. right. eapply CIH.
       hexploit match_states_intro.
       { eapply CSC1. }
-      1,2,5: eauto.
-      2:{ instantiate (1:=Kseq s0 tcont). eauto. }
-      { econs 2; eauto. clarify. }
+      3:{ instantiate (1:=Kseq s0 tcont). ss. destruct s0; eauto. eapply compile_stmt_no_Sreturn in CSC2; clarify. }
+      3:{ econs 2; eauto. clarify. }
+      all: eauto.
+      { ss. destruct s0; eauto. eapply compile_stmt_no_Sreturn in CSC2; clarify. }
       i.
       match goal with
       | [ H: match_states _ _ _ _ _ ?it0 _ |- match_states _ _ _ _ _ ?it1 _ ] =>
         replace it1 with it0; eauto
       end.
-      grind.
+      unfold itree_of_cont_stmt, itree_of_imp_cont.
+      Red.prw ltac:(_red_gen) 1 0. grind.
+
     - unfold itree_of_cont_stmt in *; unfold itree_of_imp_cont in *. rewrite interp_imp_If. sim_red. ss.
       destruct (compile_expr i) eqn:CEXPR; destruct (compile_stmt (get_gmap src) code1) eqn:CCODE1;
         destruct (compile_stmt (get_gmap src) code2) eqn:CCODE2; uo; clarify.
@@ -454,19 +410,20 @@ Section PROOF.
       sim_red. destruct rv; clarify. ss. destruct (n =? 0)%Z eqn:CZERO; ss; clarify.
       { rewrite Z.eqb_eq in CZERO. clarify.
         (* tau point *)
-        pfold. econs 4.
+        pfold. econs 6; ss.
         { admit "ez: strict_determinate_at". }
         eexists. eexists.
         { eapply step_ifthenelse; ss.
           econs; eauto.
           + econs. ss.
           + ss. }
-        unfold ordN. eexists; split; auto. eexists.
-        des_ifs. right. eapply CIH.
+        eexists. eexists.
+        { eapply step_tau. }
+        eexists. des_ifs. right. eapply CIH.
         hexploit match_states_intro; eauto. }
       { rewrite Z.eqb_neq in CZERO.
         (* tau point *)
-        pfold. econs 4.
+        pfold. econs 6; ss.
         { admit "ez: strict_determinate_at". }
         eexists. eexists.
         { eapply step_ifthenelse.
@@ -477,24 +434,31 @@ Section PROOF.
             rewrite negb_false_iff in CONTRA. apply Int64.same_if_eq in CONTRA.
             unfold to_long in CONTRA. unfold Int64.zero in CONTRA.
             admit "ez: int64 extenttionality with wf-ed values". }
-        unfold ordN. eexists; split; auto. eexists.
-        des_ifs. right. eapply CIH.
+        eexists. eexists.
+        { eapply step_tau. }
+        eexists. des_ifs. right. eapply CIH.
         hexploit match_states_intro.
         { eapply CCODE1. }
         all: eauto. }
+
     - ss. uo; des_ifs.
       unfold itree_of_cont_stmt, itree_of_imp_cont. rewrite interp_imp_CallFun.
       des_ifs; sim_red.
       { sim_triggerUB. }
+      unfold Imp2Csharpminor.compile in COMP. unfold _compile in COMP. des_ifs.
+      unfold compile_gdefs in Heq2. uo; des_ifs; clarify.
+      match goal with
+      | [ |- paco3 (_sim _ (semantics ?tp) _) _ _ _ _ ] =>
+        set (tgtp:=tp)
+      end.
       destruct rp. eapply step_exprs; eauto.
       { admit "mid: index". }
-      { admit "mid: index". }
       i. sim_red. destruct r0. destruct l0.
-      { ss. admit "mod: r_state is nil". }
-      ss. grind.
+      { ss. admit "mid?: r_state is nil". }
+      ss. grind. unfold ordN in *.
       do 3 (pfold; sim_tau; left). sim_red.
       match goal with
-      | [ |- paco4 _ _ _ _ (r0 <- unwrapU (?f);; _) _ ] => destruct f eqn:FSEM; ss
+      | [ |- paco3 _ _ _ (r0 <- unwrapU (?f);; _) _ ] => destruct f eqn:FSEM; ss
       end.
       2:{ sim_triggerUB. }
       grind.
@@ -507,32 +471,67 @@ Section PROOF.
       match goal with
       | [ FOUND: o_map (?a) _ = _ |- _ ] => destruct a eqn:FOUND2; ss; clarify
       end.
+
+      (* make lemma *)
+      assert (COMPF: exists tf0, compile_function (get_gmap src) f0 = Some tf0).
+      { admit "ez: use FOUND2". }
+      destruct COMPF as [tf0 COMPF].
+      assert (SRCF: In (f, f0) (prog_funs src)).
+      { admit "ez: trivial, use FOUND2". }
+      assert (TGTF: In (s2p f, AST.Gfun (AST.Internal tf0)) l1).
+      { admit "ez: by definition". }
+      assert (TGTFG: In (s2p f, AST.Gfun (AST.Internal tf0)) tgtp.(AST.prog_defs)).
+      { admit "mid?: need to construct tgt's genv". }
+      eapply Globalenvs.Genv.find_symbol_exists in TGTFG.
+      destruct TGTFG as [b TGTFG].
+      assert (TGTGFIND: Globalenvs.Genv.find_def (Globalenvs.Genv.globalenv tgtp) b = Some (Gfun (Internal tf0))).
+      { admit "mid? from construction of tgt's genv". }
+
+      unfold ident_key in Heq0.
+      assert (SIG: s = make_signature (Datatypes.length (Imp.fn_params f0))).
+      { admit "ez: trivial, use FOUND2". }
+      clarify.
+
+      unfold compile_function in COMPF. uo; des_ifs. rename s into bodytf0.
+      assert (COMPFRET: forall tfd0 tf0, In tfd0 l1 -> snd tfd0 = AST.Gfun (AST.Internal tf0) ->
+                                    tf0.(fn_body) = Sseq (bodytf0) (Sreturn (Some (Evar (s2p "return"))))).
+      { admit "ez: trivial by definition". }
+
       unfold cfun. sim_red. rewrite Any.upcast_downcast. sim_red.
       rewrite unfold_eval_imp_only.
       destruct (init_args (Imp.fn_params f0) rvs []) eqn:ARGS; sim_red.
       2:{ sim_triggerUB. }
       (* tau point?? need a tau BEFORE denote_stmt(fn_body) *)
-      rewrite interp_imp_bind. sim_red.
-      pfold. econs 4.
+      rewrite interp_imp_tau. sim_red.
+      pfold. econs 6; auto.
       { admit "ez: strict_determinate_at". }
       eexists. eexists.
       { eapply step_call; eauto.
         - econs. econs 2.
           { apply Maps.PTree.gempty. }
-          admit "mid: genv, use ident_key (s2p f) _ = Some _".
-        - admit "mid: genv, need smth like injection, use FOUND".
-        - admit "ez: should follow from above two". }
-      unfold ordN in *. eexists; split; auto. eexists. left.
+          eapply TGTFG.
+        - rewrite Globalenvs.Genv.find_funct_find_funct_ptr.
+          rewrite Globalenvs.Genv.find_funct_ptr_iff. ss. eapply TGTGFIND.
+        - ss. }
+
+      eexists. exists (step_tau _).
+      eexists. left.
       pfold. econs 4.
       { admit "ez: strict_determinate_at". }
       eexists. eexists.
-      { eapply step_internal_function; eauto.
+      { eapply step_internal_function; ss; eauto.
+        - econs.
         - admit "ez: need wf condition for a Imp.program & lemmas".
         - admit "ez: need wf condition for a Imp.program & lemmas".
-        - admit "ez: need wf condition for a Imp.program & lemmas".
-        - admit "ez: need wf condition for a Imp.program & lemmas, fn_vars == []".
+        - econs.
         - admit "ez: need wf condition for a Imp.program & lemmas". }
-      eexists; split; auto. eexists. grind. right.
+      eexists; split; auto. grind. left.
+
+      pfold. econs 4.
+      { admit "ez: strict_determinate_at". }
+      eexists. eexists.
+      { eapply step_seq. }
+      eexists; split; auto. right.
       eapply CIH.
       set (ge:= Sk.load_skenv (defs src)).
       set (ms:=ImpMod.modsemL src ge).
@@ -542,20 +541,23 @@ Section PROOF.
         replace i with
     (` r0 : r_state * p_state * (lenv * val) <-
      EventsL.interp_Es (prog ms)
-       (transl_all mn (interp_imp ge (denote_stmt (Imp.fn_body f0)) (init_lenv (Imp.fn_vars f0) ++ l1)))
+       (transl_all mn (interp_imp ge (denote_stmt (Imp.fn_body f0)) (init_lenv (Imp.fn_vars f0) ++ l2)))
        (c, ε :: c0 :: l0, p);; x4 <- itree_of_imp_pop ge ms mn mn x le r0;; ` x : _ <- next x4;; stack x)
       end.
-      2:{ grind. Red.prw ltac:(_red_gen) 2 0. grind. Red.prw ltac:(_red_gen) 1 0.
-          Red.prw ltac:(_red_gen) 2 0. grind. Red.prw ltac:(_red_gen) 2 0. grind.
-          Red.prw ltac:(_red_gen) 1 0. grind. }
+      2:{ rewrite interp_imp_bind. Red.prw ltac:(_red_gen) 1 0. grind.
+          Red.prw ltac:(_red_gen) 2 0. grind.
+          Red.prw ltac:(_red_gen) 2 0. Red.prw ltac:(_red_gen) 1 0. grind.
+          Red.prw ltac:(_red_gen) 2 0. Red.prw ltac:(_red_gen) 1 0. grind. }
+
       hexploit match_states_intro.
-      4:{ instantiate (1:=Kcall (Some (s2p x)) tf empty_env tle tcont). ss. econs 1. }
-      4:{ instantiate (1:= fun r0 =>
+      4:{ instantiate (1:=Kseq (Sreturn (Some (Evar (s2p "return")))) (Kcall (Some (s2p x)) tf empty_env tle tcont)). ss. }
+      5:{ instantiate (1:= fun r0 =>
                              ` x4 : r_state * p_state * (lenv * val) <- itree_of_imp_pop ge ms mn mn x le r0;;
                                     ` x0 : r_state * p_state * (lenv * val) <- next x4;; stack x0).
           instantiate (1:=mn). instantiate (1:=ms). instantiate (1:=ge). instantiate (1:=get_gmap src).
           econs 2; ss; eauto. }
-      3:eauto.
+      3: eauto.
+      1:{ eapply Heq5. }
       4:{ instantiate (9:= EventsL.interp_Es (prog ms) (transl_all mn (interp_imp ge (denote_stmt (Imp.fn_body f0)) (init_lenv (Imp.fn_vars f0) ++ l1))) (c, ε :: c0 :: l0, p)). i.
           match goal with
           | [ H1: match_states _ _ _ _ _ ?i0 _ |- match_states _ _ _ _ _ ?i1 _] =>
